cleanup RVShadowStackProperties

examples/rv/RVShadowStackProperties.v
@@ -4,24 +4,21 @@ Require Import Koika.BitsToLists Koika.Frontend Koika.UntypedSemantics
   Koika.UntypedIndSemantics Koika.UntypedIndTactics.
 Require Import Koika.SimpleFormInterpretation.
 Require Import rv.ShadowStack rv.RVCore rv.rv32 rv.rv32i.
-(* Require Import rv.RVCoreNoShadowStack rv.rv32NoShadowStack *)
-(*   rv.rv32iNoShadowStack. *)
 Require Import SimpleForm SimpleVal.
 
 Import Coq.Lists.List.ListNotations.
 Scheme Equality for list.
 
 (* We mostly reason on the instruction that is currently entering the execute
-   stage. All the information available about it is in the d2e structure
-   (decode to execute buffer). *)
+   stage. All the information available about it is in the d2e buffer. *)
 Section ShadowStackProperties.
   Context {REnv : Env RV32I.reg_t}.
   Context (ext_sigma : RV32I.ext_fn_t -> val -> val).
   Context (ext_Sigma : RV32I.ext_fn_t -> ExternalSignature).
 
   Hypothesis wt_sigma: forall (ufn : RV32I.ext_fn_t) (vc : val),
-      wt_val (arg1Sig (ext_Sigma ufn)) vc ->
-      wt_val (retSig (ext_Sigma ufn)) (ext_sigma ufn vc).
+    wt_val (arg1Sig (ext_Sigma ufn)) vc
+    -> wt_val (retSig (ext_Sigma ufn)) (ext_sigma ufn vc).
 
   Definition drules rule :=
     match uaction_to_daction (desugar_action tt (RV32I.rv_urules rule)) with
@@ -31,32 +28,29 @@ Section ShadowStackProperties.
 
   Hypothesis rules_wt:
     forall rule : rv_rules_t,
-    exists t : type, wt_daction (Sigma:=ext_Sigma) (R:=RV32I.R) unit string string [] (drules rule) t.
+    exists t : type,
+    wt_daction
+      (Sigma:=ext_Sigma) (R:=RV32I.R) unit string string [] (drules rule) t.
 
   Definition schedule := rv_schedule.
   Definition eql (l1 l2: list bool) : bool := list_beq bool Bool.eqb l1 l2.
 
   (* Propositions about the initial state *)
-  Definition no_mispred
-    (ctx: env_t REnv (fun _ : RV32I.reg_t => val))
-  : Prop :=
+  Definition no_mispred (ctx: env_t REnv (fun _ : RV32I.reg_t => val)) : Prop :=
     forall v,
     getenv REnv ctx (RV32I.d2e (RV32I.fromDecode.data0)) =
       Struct (RV32I.decode_bookkeeping) v ->
     get_field_struct (struct_fields RV32I.decode_bookkeeping) v "epoch" =
     Some (getenv REnv ctx (RV32I.epoch)).
 
-  Definition stack_empty
-    (ctx: env_t REnv (fun _ : RV32I.reg_t => val))
+  Definition stack_empty (ctx: env_t REnv (fun _ : RV32I.reg_t => val))
   : Prop :=
     getenv REnv ctx (RV32I.stack (RV32I.ShadowStack.size))
     = @val_of_value
       (bits_t RV32I.ShadowStack.index_sz)
       (Bits.of_nat (RV32I.ShadowStack.index_sz) 0).
 
-  Definition stack_full
-    (ctx: env_t REnv (fun _ : RV32I.reg_t => val))
-  : Prop :=
+  Definition stack_full (ctx: env_t REnv (fun _ : RV32I.reg_t => val)) : Prop :=
     getenv REnv ctx (RV32I.stack (RV32I.ShadowStack.size))
     = @val_of_value
       (bits_t RV32I.ShadowStack.index_sz)
@@ -109,9 +103,7 @@ Section ShadowStackProperties.
           (eql rs1 [false; false; false; false; true])
           || (eql rs1 [false; false; true; false; true])))).
 
-  Definition stack_push
-    (ctx: env_t REnv (fun _ : RV32I.reg_t => val))
-  : Prop :=
+  Definition stack_push (ctx: env_t REnv (fun _ : RV32I.reg_t => val)) : Prop :=
     forall v w b,
     getenv REnv ctx (RV32I.d2e (RV32I.fromDecode.data0)) =
       Struct (RV32I.decode_bookkeeping) v ->
@@ -121,9 +113,7 @@ Section ShadowStackProperties.
       Some (Bits b) ->
     is_call_instruction (Bits.of_N 32 (Bits.to_N (vect_of_list b))) = true.
 
-  Definition stack_pop
-    (ctx: env_t REnv (fun _ : RV32I.reg_t => val))
-  : Prop :=
+  Definition stack_pop (ctx: env_t REnv (fun _ : RV32I.reg_t => val)) : Prop :=
     forall v w b,
     getenv REnv ctx (RV32I.d2e (RV32I.fromDecode.data0)) =
       Struct (RV32I.decode_bookkeeping) v ->
@@ -154,8 +144,7 @@ Section ShadowStackProperties.
     end.
 
   (* TODO should never return None, simplify? *)
-  Definition stack_top_address
-    (ctx: env_t REnv (fun _ : RV32I.reg_t => val))
+  Definition stack_top_address (ctx: env_t REnv (fun _ : RV32I.reg_t => val))
   : option (bits_t 32) :=
     let index_raw := getenv REnv ctx (RV32I.stack RV32I.ShadowStack.size) in
     let index_nat := Bits.to_nat (vect_of_list (ubits_of_value index_raw)) in
@@ -168,17 +157,17 @@ Section ShadowStackProperties.
     | None => None
     end.
 
-  Definition stack_underflow
-    (ctx: env_t REnv (fun _ : RV32I.reg_t => val))
-  : Prop := no_mispred ctx /\ stack_empty ctx /\ stack_pop ctx.
-  Definition stack_overflow
-    (ctx: env_t REnv (fun _ : RV32I.reg_t => val))
+  Definition stack_underflow (ctx: env_t REnv (fun _ : RV32I.reg_t => val))
+  : Prop :=
+    no_mispred ctx /\ stack_empty ctx /\ stack_pop ctx.
+  Definition stack_overflow (ctx: env_t REnv (fun _ : RV32I.reg_t => val))
   : Prop :=
     no_mispred ctx /\ stack_full ctx /\ (not (stack_pop ctx)) /\ stack_push ctx.
   Definition stack_address_violation
     (ctx: env_t REnv (fun _ : RV32I.reg_t => val))
   : Prop :=
-    no_mispred ctx /\ stack_push ctx /\ stack_top_address ctx <> stack_push_address ctx.
+    no_mispred ctx /\ stack_push ctx
+    /\ stack_top_address ctx <> stack_push_address ctx.
 
   Definition stack_violation
     (ctx: env_t REnv (fun _ : RV32I.reg_t => val))
@@ -186,45 +175,22 @@ Section ShadowStackProperties.
     stack_underflow ctx \/ stack_overflow ctx \/ stack_address_violation ctx.
 
   (* Final state *)
-  Definition halt_set
-    (ctx: env_t REnv (fun _ : RV32I.reg_t => val))
+  Definition halt_set (ctx: env_t REnv (fun _ : RV32I.reg_t => val))
   : Prop :=
     forall ctx',
     UntypedIndSemantics.interp_cycle
       RV32I.rv_urules ctx ext_sigma schedule ctx' ->
     getenv REnv ctx' RV32I.halt = @val_of_value (bits_t 1) Ob~1.
 
-  Fixpoint interp_n_cycles
-    n (ctx: env_t REnv (fun _ : RV32I.reg_t => val))
+  Fixpoint interp_n_cycles n (ctx: env_t REnv (fun _ : RV32I.reg_t => val))
   : env_t REnv (fun _ : RV32I.reg_t => val) :=
     match n with
     | O => ctx
-    | S n' => interp_n_cycles n' (
-        UntypedSemantics.interp_cycle RV32I.rv_urules ctx ext_sigma schedule
-      )
+    | S n' =>
+      interp_n_cycles
+        n'
+        (UntypedSemantics.interp_cycle RV32I.rv_urules ctx ext_sigma schedule)
     end.
-
-  (* Fixpoint interp_n_cycles_no_shadow_stack *)
-  (*   n (ctx: env_t REnv (fun _ : RV32I.reg_t => val)) *)
-  (* : env_t REnv (fun _ : RV32I.reg_t => val) := *)
-  (*   match n with *)
-  (*   | O => ctx *)
-  (*   | S n' => interp_n_cycles n' ( *)
-  (*       UntypedSemantics.interp_cycle RV32I.rv_urules ctx ext_sigma schedule *)
-  (*     ) *)
-  (*   end. *)
-
-  (* Definition is_sink_state *)
-  (*   (ctx: env_t REnv (fun _ : RV32I.reg_t => val)) *)
-  (* : Prop := *)
-  (*   forall n ctx', interp_n_cycles n ctx' = ctx. *)
-
-  (* Main lemmas *)
-  (* Lemma halt_leads_to_a_sink_state: *)
-  (*   forall (ctx: env_t REnv (fun _ : RV32I.reg_t => val)), *)
-  (*   halt_set ctx -> is_sink_state ctx. *)
-  (* Proof. *)
-  (* Qed. *)
 
   Ltac destr_in H :=
     match type of H with
@@ -237,8 +203,7 @@ Section ShadowStackProperties.
     end.
 
   Definition is_write_halt
-    (reg_t ext_fn_t: Type)
-    (ua: uaction pos_t var_t fn_name_t reg_t ext_fn_t)
+    (reg_t ext_fn_t: Type) (ua: uaction pos_t var_t fn_name_t reg_t ext_fn_t)
     (fR: reg_t -> RV32I.reg_t) (fSigma: ext_fn_t -> RV32I.ext_fn_t)
   : bool :=
     match ua with
@@ -250,652 +215,50 @@ Section ShadowStackProperties.
     | _ => false
     end.
 
-  Set Typeclasses Debug.
   Instance eq_dec_reg: EqDec RV32I.reg_t := EqDec_FiniteType.
   Existing Instance etaRuleInformationRaw.
 
   Ltac inv H := inversion H; try subst; clear H.
 
-
-  Definition simplify_sf  sf ctx :=
-    {|
-      final_values := final_values sf;
-      vars := Maps.PTree.map (fun _ '(t,a) => (t, simplify_sact (REnv:=REnv) (reg_t:=RV32I.reg_t) ctx ext_sigma a)) (vars sf)
-
+  Definition simplify_sf  sf ctx := {|
+    final_values := final_values sf;
+    vars :=
+      Maps.PTree.map
+        (fun _ '(t,a) => (
+          t,
+          simplify_sact (REnv := REnv) (reg_t := RV32I.reg_t) ctx ext_sigma a
+        ))
+        (vars sf)
     |}.
 
   Definition halt_set2 ctx :=
     forall sf n,
-      remove_vars_for_var (simplify_sf (schedule_to_simple_form RV32I.R (Sigma:=ext_Sigma)
-                                           drules schedule) ctx) RV32I.halt = Some sf ->
-      list_assoc (final_values sf) RV32I.halt = Some n ->
-      SimpleForm.interp_sact REnv ctx (vars sf) (sigma:=ext_sigma) (SVar n) (Bits [true]).
-
-
-  Lemma wt_sact_simplify_sact:
-    forall vvs ctx
-           (WTRENV: Wt.wt_renv RV32I.R REnv ctx) a t,
-      (* wt_vvs RV32I.R (Sigma:=ext_Sigma) (vars sf) -> *)
-      wt_sact RV32I.R (Sigma:=ext_Sigma) vvs a t ->
-      wt_sact RV32I.R (Sigma:=ext_Sigma) vvs (simplify_sact ctx ext_sigma a) t.
-  Proof.
-    induction a; simpl; intros; eauto.
-    - inv H. destr. 2: econstructor; eauto.
-      repeat destr; try now (econstructor; eauto). subst. eauto. eauto.
-    - inv H. destr; try now econstructor; eauto.
-      repeat destr; try now (econstructor; eauto). subst. inv H4. econstructor. econstructor.
-      eapply eval_sact_no_vars_wt in Heqo. 4: apply IHa; eauto. inv Heqo. reflexivity.
-      auto. auto.
-    - inv H. destr; try now econstructor; eauto.
-      destr; try now (econstructor; eauto).
-      + inv H6.
-        destruct (eval_sact_no_vars ctx ext_sigma (simplify_sact ctx ext_sigma a1)) eqn:?.
-        generalize (eval_sact_no_vars_wt RV32I.R ext_Sigma ctx ext_sigma (wt_sigma:=wt_sigma)
-                                         WTRENV _ _ _ (IHa1 _ H3) _ Heqo). intro WT1. inv WT1.
-        * destruct (eval_sact_no_vars ctx ext_sigma (simplify_sact ctx ext_sigma a2)) eqn:?.
-          generalize (eval_sact_no_vars_wt RV32I.R ext_Sigma ctx ext_sigma (wt_sigma:=wt_sigma)
-                                           WTRENV _ _ _ (IHa2 _ H5) _ Heqo0). intro WT2. inv WT2.
-          repeat destr; repeat econstructor; eauto.
-          repeat destr; repeat econstructor; eauto.
-        * destruct (eval_sact_no_vars ctx ext_sigma (simplify_sact ctx ext_sigma a2)) eqn:?.
-          generalize (eval_sact_no_vars_wt RV32I.R ext_Sigma ctx ext_sigma (wt_sigma:=wt_sigma)
-                                           WTRENV _ _ _ (IHa2 _ H5) _ Heqo0). intro WT2. inv WT2.
-          repeat destr; repeat econstructor; eauto.
-          repeat destr; repeat econstructor; eauto.
-      + inv H6.
-        destruct (eval_sact_no_vars ctx ext_sigma (simplify_sact ctx ext_sigma a1)) eqn:?.
-        generalize (eval_sact_no_vars_wt RV32I.R ext_Sigma ctx ext_sigma (wt_sigma:=wt_sigma)
-                                         WTRENV _ _ _ (IHa1 _ H3) _ Heqo). intro WT1. inv WT1.
-        * destruct (eval_sact_no_vars ctx ext_sigma (simplify_sact ctx ext_sigma a2)) eqn:?.
-          generalize (eval_sact_no_vars_wt RV32I.R ext_Sigma ctx ext_sigma (wt_sigma:=wt_sigma)
-                                           WTRENV _ _ _ (IHa2 _ H5) _ Heqo0). intro WT2. inv WT2.
-          repeat destr; repeat econstructor; eauto.
-          repeat destr; repeat econstructor; eauto.
-        * destruct (eval_sact_no_vars ctx ext_sigma (simplify_sact ctx ext_sigma a2)) eqn:?.
-          generalize (eval_sact_no_vars_wt RV32I.R ext_Sigma ctx ext_sigma (wt_sigma:=wt_sigma)
-                                           WTRENV _ _ _ (IHa2 _ H5) _ Heqo0). intro WT2. inv WT2.
-          repeat destr; repeat econstructor; eauto.
-          repeat destr; repeat econstructor; eauto.
-    - inv H. econstructor. eauto.
-  Qed.
-
-  Lemma wt_sact_simplify_vars:
-    forall vvs ctx
-           (WTRENV: Wt.wt_renv RV32I.R REnv ctx) a t,
-      (* wt_vvs RV32I.R (Sigma:=ext_Sigma) (vars sf) -> *)
-      wt_sact RV32I.R (Sigma:=ext_Sigma) vvs a t ->
-      wt_sact RV32I.R (Sigma:=ext_Sigma) (Maps.PTree.map (fun _ '(t,a) => (t, simplify_sact ctx ext_sigma a )) vvs) a t.
-  Proof.
-    induction a; simpl; intros; eauto.
-    - inv H. econstructor; eauto.
-      rewrite Maps.PTree.gmap. setoid_rewrite H1. reflexivity.
-    - inv H; econstructor; eauto.
-    - inv H. econstructor; eauto.
-    - inv H. econstructor; eauto.
-    - inv H. econstructor; eauto.
-    - inv H. econstructor; eauto.
-    - inv H. econstructor; eauto.
-  Qed.
-
-  Lemma wt_vvs_simplify_sf:
-    forall sf ctx
-           (WTRENV: Wt.wt_renv RV32I.R REnv ctx),
-      wt_vvs RV32I.R (Sigma:=ext_Sigma) (vars sf) ->
-      wt_vvs RV32I.R (Sigma:=ext_Sigma) (vars (simplify_sf sf ctx)).
-  Proof.
-    red; intros. simpl in H0.
-    rewrite Maps.PTree.gmap in H0.
-    unfold option_map in H0; repeat destr_in H0; inv H0.
-    eapply H in Heqo. simpl.
-    eapply wt_sact_simplify_vars. auto.
-    eapply wt_sact_simplify_sact; eauto.
-  Qed.
-
-  Lemma vsv_simplify_sf:
-    forall sf ctx,
-      vvs_smaller_variables (vars sf) ->
-      vvs_smaller_variables (vars (simplify_sf sf ctx)).
-  Proof.
-    red; intros. simpl in H0.
-    rewrite Maps.PTree.gmap in H0.
-    unfold option_map in H0; repeat destr_in H0; inv H0.
-    eapply H in Heqo. eapply Heqo.
-
-
-    Lemma var_in_sact_simplify_sact:
-      forall ctx s v,
-        var_in_sact (simplify_sact (REnv:=REnv) ctx ext_sigma s) v ->
-        var_in_sact s v.
-    Proof.
-      intros ctx s v VIS.
-      apply var_in_sact_ok in VIS.
-      eapply var_in_sact_ok_inv. apply RV32I.R. apply ext_Sigma.
-      revert s v VIS.
-      induction s; simpl; intros; eauto.
-      - rewrite ! in_app_iff. repeat destr_in VIS; eauto.
-        + simpl in VIS. rewrite ! in_app_iff in VIS. intuition eauto.
-        + simpl in VIS. rewrite ! in_app_iff in VIS. intuition eauto.
-        + simpl in VIS. rewrite ! in_app_iff in VIS. intuition eauto.
-        + simpl in VIS. rewrite ! in_app_iff in VIS. intuition eauto.
-        + simpl in VIS. rewrite ! in_app_iff in VIS. intuition eauto.
-        + simpl in VIS. rewrite ! in_app_iff in VIS. intuition eauto.
-        + simpl in VIS. rewrite ! in_app_iff in VIS. intuition eauto.
-      - repeat destr_in VIS; eauto. inv VIS.
-      - rewrite ! in_app_iff. repeat destr_in VIS; eauto.
-        all: try (simpl in VIS; rewrite ! in_app_iff in VIS; intuition eauto).
-        all: try now (inv VIS).
-        Unshelve. apply RV32I.R.
-    Qed.
-    eapply var_in_sact_simplify_sact. eauto.
-  Qed.
+    remove_vars_for_var
+      (simplify_sf
+        (schedule_to_simple_form RV32I.R (Sigma:=ext_Sigma) drules schedule) ctx
+      )
+      RV32I.halt
+    = Some sf
+    -> list_assoc (final_values sf) RV32I.halt = Some n
+    -> SimpleForm.interp_sact
+         REnv ctx (vars sf) (sigma:=ext_sigma) (SVar n) (Bits [true]).
 
   Lemma stack_violation_results_in_halt:
-    (* forall (env_bf env_af: @UREnv RV32I.reg_t REnv), *)
-    (* (env_af = SimpleFormInterpretation.interp_cycle env_bf ext_sigma ) -> True. *)
-    forall ctx
-           (WTRENV: Wt.wt_renv RV32I.R REnv ctx)
-           (NoHalt: (getenv REnv ctx RV32I.halt) = Bits [false])
-           (Valid: getenv REnv ctx (RV32I.d2e RV32I.fromDecode.valid0) = Bits [true])
-           (Legal:
-             forall v v2,
-               getenv REnv ctx (RV32I.d2e RV32I.fromDecode.data0) =
-                 Struct RV32I.decode_bookkeeping v ->
-               get_field_struct (struct_fields RV32I.decode_bookkeeping) v "dInst" = Some (Struct decoded_sig v2) ->
-               get_field_struct (struct_fields decoded_sig) v2 "legal" = Some (Bits [true]))
-
-    ,
+    forall
+      ctx (WTRENV: Wt.wt_renv RV32I.R REnv ctx)
+      (NoHalt: (getenv REnv ctx RV32I.halt) = Bits [false])
+      (Valid: getenv REnv ctx (RV32I.d2e RV32I.fromDecode.valid0) = Bits [true])
+      (Legal:
+        forall v v2,
+        getenv REnv ctx (RV32I.d2e RV32I.fromDecode.data0)
+        = Struct RV32I.decode_bookkeeping v
+        -> get_field_struct
+             (struct_fields RV32I.decode_bookkeeping) v "dInst"
+        = Some (Struct decoded_sig v2
+        -> get_field_struct (struct_fields decoded_sig) v2 "legal"
+        = Some (Bits [true])),
     stack_violation ctx -> halt_set2 ctx.
   Proof.
-    intros ctx WTRENV NoHalt Valid Legal SV.
-    unfold halt_set2. intros sf n SF HALT.
-    unfold stack_violation in SV.
-    unfold stack_underflow, stack_overflow, stack_address_violation in SV.
-
-    generalize (WTRENV (RV32I.d2e RV32I.fromDecode.data0)). intro WTdata0. simpl in WTdata0.
-    inv WTdata0.
-    assert (NMP: no_mispred ctx) by intuition.
-    symmetry in H0. specialize (NMP _ H0).
-    generalize (WTRENV RV32I.epoch). intro WTepoch. simpl in WTepoch.
-    apply Sact.wt_val_bool in WTepoch. destruct WTepoch as (? & WTepoch). rewrite WTepoch in NMP.
-
-    assert (WTsize:= WTRENV (RV32I.stack RV32I.ShadowStack.size)). simpl in WTsize. inv WTsize.
-    change (log2 5) with 3 in H3.
-    destruct bs. simpl in H3; lia.
-    destruct bs. simpl in H3; lia.
-    destruct bs. simpl in H3; lia.
-    destruct bs. 2: simpl in H3; lia. clear H3.
-    symmetry in H2. simpl in H1.
-    
-    Ltac invtypes := repeat match goal with
-           | H: Forall2 _ [] _ |- _ => inv H
-           | H: Forall2 _ (_::_) _ |- _ =>
-               inv H
-           | H: wt_val (bits_t 1) _ |- _ => apply Sact.wt_val_bool in H; destruct H; subst
-                            end.
-    invtypes.
-    inv H6.
-    simpl in H1. invtypes.
-    simpl in NMP. inv NMP.
-
-    assert (EQse:
-        stack_empty ctx <->
-        b = false /\ b0 = false /\ b1 = false
-           ).
-    unfold stack_empty. rewrite H2. simpl. cbv. intuition congruence.
-
-    inv H11.
-    assert (EQspop: stack_pop ctx <-> is_ret_instruction
-                                        (Bits.of_N 32 (Bits.to_N (Bits.of_list bs))) = true).
-    unfold stack_pop. rewrite H0.
-    split. intro A. eapply A. eauto. simpl. eauto. simpl. auto.
-    intros IRI v w b2 EQ1 EQ2 EQ3. inv EQ1; simpl in EQ2; inv EQ2; simpl in EQ3; inv EQ3. auto.
-
-    assert (EQspush: stack_push ctx <-> is_call_instruction
-                                        (Bits.of_N 32 (Bits.to_N (Bits.of_list bs))) = true).
-    unfold stack_push. rewrite H0.
-    split. intro A. eapply A. eauto. simpl. eauto. simpl. auto.
-    intros ICI v w b2 EQ1 EQ2 EQ3. inv EQ1; simpl in EQ2; inv EQ2; simpl in EQ3; inv EQ3. auto.
-
-    assert (EQsf:
-             stack_full ctx <->
-               b = false /\ b0 = false /\ b1 = true
-           ).
-    unfold stack_full. rewrite H2. simpl. cbv. intuition congruence.
-    inv H4.
-    assert (EQpa: stack_push_address ctx =
-              Some (Bits.of_N 32 (Bits.to_N (Bits.of_list bs0) + 4)%N)
-           ).
-    {
-      unfold stack_push_address.
-      rewrite H0. simpl. auto.
-    }
-    assert (Bits.to_nat Ob~b1~b0~b < pow2 RV32I.ShadowStack.index_sz).
-    change (Bits.to_nat Ob~b1~b0~b < pow2 3). simpl.
-    apply Bits.to_nat_bounded.
-    edestruct @index_of_nat_bounded as (idx & EQidx). apply H.
-
-    assert (WTtop:= WTRENV (RV32I.stack (RV32I.ShadowStack.stack idx))). simpl in WTtop.
-    inv WTtop.
-
-    assert (EQta: stack_top_address ctx =
-                    Some (Bits.of_N 32 (Bits.to_N (Bits.of_list bs1)))
-           ).
-    {
-      unfold stack_top_address.
-      rewrite H2. simpl ubits_of_value.
-      simpl Bits.of_list.
-      setoid_rewrite EQidx. rewrite <- H6. reflexivity.
-    }
-
-    move SV at bottom.
-    assert (CONDS:
-             stack_empty ctx /\ stack_pop ctx
-             \/ stack_push ctx /\ ((stack_full ctx /\ ~ stack_pop ctx) \/ stack_top_address ctx <> stack_push_address ctx)).
-    now intuition. clear SV.
-    rewrite EQse, EQspop, EQspush, EQsf, EQpa, EQta in CONDS.
-    clear EQse EQspop EQspush EQsf EQpa EQta.
-    move Legal at bottom.
-    specialize (fun w => Legal _ w H0). simpl in Legal.
-    specialize (Legal _ eq_refl). simpl in Legal. inv Legal.
-
-
-    Ltac replacereg H sf :=
-      let sf2 := fresh "sf" in
-      match type of H with
-        getenv _ _ ?r = ?v =>
-          set (sf2 := replace_reg sf r v)
-      | ?v = getenv _ _ ?r =>
-          set (sf2 := replace_reg sf r v)
-      end.
-    replacereg NoHalt sf.
-    replacereg Valid sf0.
-    replacereg H0 sf1.
-    replacereg WTepoch sf2.
-    replacereg H2 sf3.
-
-    assert (interp_sact (sigma:=ext_sigma) REnv ctx (vars sf4) (SVar n) (Bits [true])).
-    Set Printing Depth 20.
-    Time native_compute in SF. injection SF. clear SF. intro A.
-    subst sf.
-    Time native_compute in sf4.
-    clear sf0 sf1 sf2 sf3.
-
-    set (ks:= PosSort.sort (map fst (Maps.PTree.elements (vars sf4)))).
-    native_compute in ks.
-    set (ks2 := firstn 21 ks). native_compute in ks2. clear ks.
-
-    set (ip := snd (fold_left
-                 (fun '(sf0, l) (var : positive) =>
-                    let '(sf1, l1) := simplify_var ctx ext_sigma sf0 var in (sf1, l1 ++ l)) ks2 (sf4,[]))).
-
-    Eval native_compute in Maps.PTree.get 117 (vars sf4).
-    Time Eval native_compute in match ip with l => List.length l end.
-
-    Eval native_compute in Maps.PTree.get 849 (vars sf4).
-
-    set (sf5 := simplify_sf sf4 ctx).
-    Time native_compute in sf5.
-    Time Eval native_compute in vvs_size (vars sf4) 2000.
-    Time Eval native_compute in vvs_size (vars sf5) 2000.
-    native_compute in H1. apply Some_inj in H1. subst n.
-    Time Eval native_compute in List.length (Maps.PTree.elements (vars sf2)).
-    
-    
-    set (sf2 := replace_reg sf RV32I.halt (Bits [false])).
-    set (sf3 := replace_reg sf2 )
-    fold sf2 in H1.
-
-
-
-    Set Printing Depth 20.
-    Time native_compute in H0. injection H0. clear H0. intro A. subst sf.
-    native_compute in H1. apply Some_inj in H1. subst n.
-    Time Eval native_compute in List.length (Maps.PTree.elements (vars sf2)).
-
-
-
-
-
-    unfold stack_violation in H.
-    unfold stack_underflow, stack_overflow, stack_address_violation in H.
-
-    assert (NMP: no_mispred ctx) by intuition.
-
-    generalize (WTRENV (RV32I.d2e RV32I.fromDecode.data0)). intro WTdata0. simpl in WTdata0.
-    inv WTdata0.
-    symmetry in H1. specialize (NMP _ H1).
-    generalize (WTRENV RV32I.epoch). intro WTepoch. simpl in WTepoch.
-    apply Sact.wt_val_bool in WTepoch. destruct WTepoch as (? & WTepoch). rewrite WTepoch in NMP.
-
-    assert (WTsize:= WTRENV (RV32I.stack RV32I.ShadowStack.size)). simpl in WTsize. inv WTsize.
-    change (log2 5) with 3 in H4.
-    destruct bs. simpl in H4; lia.
-    destruct bs. simpl in H4; lia.
-    destruct bs. simpl in H4; lia.
-    destruct bs. 2: simpl in H4; lia. clear H4.
-    symmetry in H3. simpl in H2.
-    Ltac invtypes := repeat match goal with
-           | H: Forall2 _ [] _ |- _ => inv H
-           | H: Forall2 _ (_::_) _ |- _ =>
-               inv H
-           | H: wt_val (bits_t 1) _ |- _ => apply Sact.wt_val_bool in H; destruct H; subst
-                            end.
-    invtypes.
-    inv H7.
-    simpl in H2. invtypes.
-    simpl in NMP. inv NMP.
-
-    assert (EQse:
-        stack_empty ctx <->
-        b = false /\ b0 = false /\ b1 = false
-           ).
-    unfold stack_empty. rewrite H3. simpl. cbv. intuition congruence.
-
-    inv H12.
-    assert (EQspop: stack_pop ctx <-> is_ret_instruction
-                                        (Bits.of_N 32 (Bits.to_N (Bits.of_list bs))) = true).
-    unfold stack_pop. rewrite H1.
-    split. intro A. eapply A. eauto. simpl. eauto. simpl. auto.
-    intros. inv H6. simpl in H7. inv H7. simpl in H10. inv H10. auto.
-
-    assert (EQspush: stack_push ctx <-> is_call_instruction
-                                        (Bits.of_N 32 (Bits.to_N (Bits.of_list bs))) = true).
-    unfold stack_push. rewrite H1.
-    split. intro A. eapply A. eauto. simpl. eauto. simpl. auto.
-    intros. inv H6. simpl in H7. inv H7. simpl in H10. inv H10. auto.
-
-    assert (EQsf:
-             stack_full ctx <->
-               b = false /\ b0 = false /\ b1 = true
-           ).
-    unfold stack_full. rewrite H3. simpl. cbv. intuition congruence.
-    inv H5.
-    assert (EQpa: stack_push_address ctx =
-              Some (Bits.of_N 32 (Bits.to_N (Bits.of_list bs0) + 4)%N)
-           ).
-    {
-      unfold stack_push_address.
-      rewrite H1. simpl. auto.
-    }
-    assert (Bits.to_nat Ob~b1~b0~b < pow2 RV32I.ShadowStack.index_sz).
-    change (Bits.to_nat Ob~b1~b0~b < pow2 3). simpl.
-    apply Bits.to_nat_bounded.
-    edestruct @index_of_nat_bounded as (idx & EQidx). apply H0.
-
-    assert (WTtop:= WTRENV (RV32I.stack (RV32I.ShadowStack.stack idx))). simpl in WTtop.
-    inv WTtop.
-
-    assert (EQta: stack_top_address ctx =
-                    Some (Bits.of_N 32 (Bits.to_N (Bits.of_list bs1)))
-           ).
-    {
-      unfold stack_top_address.
-      rewrite H3. simpl ubits_of_value.
-      simpl Bits.of_list.
-      setoid_rewrite EQidx. rewrite <- H7. reflexivity.
-    }
-
-    move H at bottom.
-    assert (CONDS:
-             stack_empty ctx /\ stack_pop ctx
-             \/ stack_push ctx /\ ((stack_full ctx /\ ~ stack_pop ctx) \/ stack_top_address ctx <> stack_push_address ctx)).
-    now intuition. clear H.
-    rewrite EQse, EQspop, EQspush, EQsf, EQpa, EQta in CONDS.
-    clear EQse EQspop EQspush EQsf EQpa EQta.
-    move Legal at bottom.
-    specialize (fun w => Legal _ w H1). simpl in Legal.
-    specialize (Legal _ eq_refl). simpl in Legal. inv Legal.
-
-    
-    econstructor.
-    native_compute. exact eq_refl.
-    econstructor.
-    econstructor. native_compute. exact eq_refl.
-    
-
-    
-
-
-
-
-
-
-
-    edestruct @schedule_to_simple_form_ok as (WTVVS & VSV & _).
-    apply wt_sigma. apply WTRENV. instantiate (1:=schedule). repeat constructor. reflexivity.
-    apply rules_wt. apply WTRENV.
-    assert (WTVVS2: wt_vvs RV32I.R (Sigma:=ext_Sigma) (vars sf2)).
-    eapply wt_vvs_simplify_sf. apply WTRENV. eauto.
-    assert (VSV2 : vvs_smaller_variables (vars sf2)).
-    eapply vsv_simplify_sf. eauto.
-    Time native_compute in sf2.
-    native_compute in H1. apply Some_inj in H1. subst n.
-    econstructor.
-    native_compute. exact eq_refl.
-    Set Printing Depth 20.
-
-    Eval native_compute in Maps.PTree.get 1788 (vars sf2).
-    Eval native_compute in Maps.PTree.get 991 (vars sf2).
-    Eval native_compute in Maps.PTree.get 13 (vars sf2).
-
-    set (sf3 :=inlining_pass sf2).
-
-    set (sf3 := replace_all_occurrences sf2 )
-    (* set (vv :=fold_left *)
-    (*             (fun (t : Maps.PTree.t (type * sact)) (n : positive) => *)
-    (*                match Maps.PTree.get n (vars sf2) with *)
-    (*                | Some v => Maps.PTree.set n v t *)
-    (*                | None => t *)
-    (*                end) (reachable_vars_aux (vars sf2) 1789 [] 1790) *)
-    (*             (Maps.PTree.empty (type * sact))). *)
-    (* Time native_compute in vv. *)
-
-
-    (* Time Eval native_compute in List.length (Maps.PTree.elements vv). *)
-
-    (* Time Eval native_compute in List.length (Maps.PTree.elements (vars sf2)). *)
-    (* Time Eval native_compute in List.length (Maps.PTree.elements (vars (remove_vars sf2))). *)
-
-    (* remove_vars *)
-    econstructor.
-    econstructor. native_compute; reflexivity.
-    econstructor. econstructor.
-    econstructor. native_compute; reflexivity.
-    econstructor.
-    constructor. simpl.
-    rewrite NoHalt. transitivity (Some (Bits [false])).
-    clear. destruct val_eq_dec. inv e. auto. reflexivity.
-    econstructor.
-    econstructor.
-    econstructor. native_compute; reflexivity.
-    econstructor.
-    rewrite Valid. simpl. reflexivity.
-    instantiate (1:=Bits[false]). 2: simpl; reflexivity. 2: reflexivity.
-    econstructor.
-    econstructor.
-    econstructor.
-    econstructor.
-    native_compute; reflexivity.
-    econstructor.
-    native_compute; reflexivity.
-    econstructor. rewrite H2. simpl. reflexivity.
-    econstructor.
-    native_compute; reflexivity.
-    econstructor. rewrite WTepoch. simpl.
-    instantiate (1:=Bits [true]). clear. destr; auto.
-    instantiate (1:=Bits [false]). 2: reflexivity.
-    {
-      econstructor.
-      econstructor. econstructor. econstructor.
-      econstructor. native_compute; reflexivity.
-      econstructor. econstructor. native_compute; reflexivity.
-      econstructor. native_compute; reflexivity.
-      econstructor. rewrite H2; simpl. reflexivity.
-      simpl; reflexivity. constructor.
-      simpl. clear. destruct val_eq_dec; try congruence. eauto.
-      simpl. eauto.
-      instantiate (1:=Bits[false]). 2: reflexivity.
-      econstructor. econstructor. econstructor.
-      econstructor. econstructor. econstructor.
-      econstructor. econstructor. native_compute; reflexivity.
-      econstructor. native_compute; reflexivity.
-      econstructor. econstructor. native_compute; reflexivity.
-      econstructor. native_compute; reflexivity.
-      econstructor. rewrite H2. simpl; eauto.
-      simpl; eauto. econstructor. simpl. eauto. constructor.
-      Eval native_compute in Bits.to_nat Ob~0~0~1~1~0.
-      assert (is_ret_instruction (Bits.of_N 32 (Bits.to_N (Bits.of_list bs))) = true \/
-                is_call_instruction (Bits.of_N 32 (Bits.to_N (Bits.of_list bs))) = true).
-      { clear - CONDS. intuition. }
-      {
-        instantiate (1:=Bits [true]). clear -H H3.
-        assert (eql (firstn 3 (skipn 4 (vect_to_list (bits_of_value (tau:=bits_t 32) (Bits.of_N 32 (Bits.to_N (Bits.of_list bs))))))) [true; true; false] = true).
-        unfold is_ret_instruction, is_call_instruction in H.
-        repeat rewrite andb_true_iff in H.
-        intuition. clear H.
-        Lemma eql_eq:
-          forall l1 l2,
-            eql l1 l2 = true -> l1 = l2.
-        Proof.
-          induction l1; simpl; intros; eauto.
-          destruct l2; congruence.
-          destruct l2. congruence.
-          rewrite andb_true_iff in H. destruct H. apply eqb_prop in H. subst. f_equal. eauto.
-        Qed.
-        apply eql_eq in H0.
-        Set Printing Depth 40.
-        rewrite <- (Bits.to_N_rew _ H3) in H0.
-        rewrite Bits.of_N_to_N in H0.
-        simpl bits_of_value in H0.
-        rewrite vect_to_list_eq_rect in H0.
-        rewrite vect_to_list_of_list in H0.
-        simpl in H0.
-        destruct bs. congruence.
-        destruct bs. congruence.
-        destruct bs. congruence.
-        destruct bs. congruence.
-        destruct bs. congruence.
-        destruct bs. congruence.
-        destruct bs. congruence.
-        inv H0. simpl. destruct val_eq_dec; try congruence.
-      }
-      econstructor. econstructor.
-      econstructor. econstructor.
-      native_compute; reflexivity.
-      econstructor. native_compute; reflexivity.
-      Set Printing Depth 20.
-      econstructor. econstructor.
-      native_compute; reflexivity.
-      econstructor. native_compute; reflexivity.
-      econstructor.
-      rewrite H2; simpl; eauto. simpl; eauto. constructor.
-      simpl. eauto. constructor. simpl.
-      change (Bits.to_nat Ob~0~0~0~1~1) with 3%nat.
-      instantiate (1:=Bits [false]).
-      Set Printing Depth 100.
-      rewrite H3. simpl.
-      assert (is_ret_instruction (Bits.of_N 32 (Bits.to_N (Bits.of_list bs))) = true \/
-                is_call_instruction (Bits.of_N 32 (Bits.to_N (Bits.of_list bs))) = true).
-      { clear - CONDS. intuition. }
-      Set Printing Depth 20.
-      {
-        clear -H H3.
-        assert (eql (firstn 3 (skipn 4 (vect_to_list (bits_of_value (tau:=bits_t 32) (Bits.of_N 32 (Bits.to_N (Bits.of_list bs))))))) [true; true; false] = true).
-        unfold is_ret_instruction, is_call_instruction in H.
-        repeat rewrite andb_true_iff in H.
-        intuition. clear H.
-        apply eql_eq in H0.
-        rewrite <- (Bits.to_N_rew _ H3) in H0.
-        rewrite Bits.of_N_to_N in H0.
-        simpl bits_of_value in H0.
-        rewrite vect_to_list_eq_rect in H0.
-        rewrite vect_to_list_of_list in H0.
-        simpl in H0.
-        destruct bs. congruence.
-        destruct bs. congruence.
-        destruct bs. congruence.
-        destruct bs. congruence.
-        destruct bs. congruence.
-        destruct bs. congruence.
-        destruct bs. congruence.
-        inv H0. simpl. destruct val_eq_dec; try congruence.
-      }
-      simpl; reflexivity.
-    }
-    simpl orb.
-    cbv iota.
-    econstructor.
-    native_compute; reflexivity.
-    econstructor.
-    econstructor.
-    native_compute; reflexivity.
-    econstructor. econstructor.
-    econstructor.
-    native_compute; reflexivity.
-    econstructor.
-    native_compute; reflexivity.
-    econstructor. rewrite H2. simpl. reflexivity.
-    econstructor.
-    native_compute; reflexivity.
-    econstructor. rewrite WTepoch.
-    instantiate (1:=true). clear. simpl; destr; auto.
-    cbv iota.
-    econstructor. native_compute; reflexivity.
-    econstructor.
-    econstructor. native_compute; reflexivity.
-    econstructor. econstructor.
-    econstructor. native_compute; reflexivity.
-    econstructor.
-    econstructor. native_compute; reflexivity.
-    econstructor. native_compute; reflexivity.
-    econstructor. rewrite H2. simpl. reflexivity.
-    simpl. reflexivity. constructor.
-    simpl. instantiate (1:= negb x0).
-    clear. destr. clear Heqs. inv e. reflexivity. clear Heqs.
-    destruct x0; simpl; congruence.
-    AAA
-    rewrite H2. simpl. reflexivity.
-    econstructor.
-    native_compute; reflexivity.
-    econstructor. rewrite WTepoch. simpl.
-    
-    simpl.
-    Eval native_compute in Maps.PTree.get 96 (vars sf2).
-
-
-
-    
-    AAA
-    simpl.
-    dependent destruction H0. dependent destruction H0.
-    dependent destruction H0. dependent destruction H0.
-    dependent destruction H1. dependent destruction H1.
-    dependent destruction H2. dependent destruction H2.
-    dependent destruction H3. dependent destruction H3.
-    dependent destruction H4. dependent destruction H4.
-    dependent destruction H5. dependent destruction H5.
-    dependent destruction H6. dependent destruction H6.
-    dependent destruction H7. dependent destruction H7.
-    dependent destruction H8. dependent destruction H8.
-    dependent destruction H9. dependent destruction H9.
-    move l1 before l0. move l2 before l1. move l3 before l2. move l4 before l3.
-    move l5 before l4. move l6 before l5. move l7 before l6. move l8 before l7.
-    move l9 before l8.
-    dependent destruction H10.
-
-    (* update_on_off *)
-    unfold RV32I.update_on_off in H0.
-    dependent destruction H0.
-    invert_full H0.
-
-    (* writeback *)
-    unfold RV32I.writeback in H1.
-    dependent destruction H1.
-    invert_full H0.
-    simpl in H38. injection H38 as H38.
-    destruct (getenv REnv ctx RV32I.halt). cbn in H40.
-    destruct (val_eq_dec (Bits sz v0) (Bits 1 [true])) in H40.
-    subst.
   Qed.
 
   Lemma no_stack_violation_behaves_as_if_no_stack:
